IMP-/IMP_Minus_Nat_Bijection.thy
@@ -1,0 +1,139 @@
+\<^marker>\<open>creator Florian Kessler\<close>
+
+theory IMP_Minus_Nat_Bijection
+  imports Multiplication "HOL-Library.Nat_Bijection" 
+    "../Cook_Levin/IMP-_To_SAS+/IMP-_To_IMP--/Primitives"
+begin
+
+definition IMP_Minus_triangle where "IMP_Minus_triangle \<equiv>
+  ''b'' ::= ((V ''a'') \<oplus> (N 1)) ;;
+  IMP_minus_mul ;;
+  ''triangle'' ::= ((V ''c'') \<then>) ;;
+  ''c'' ::= (A (N 0))"
+
+lemma IMP_Minus_triangle_correct: 
+   "(IMP_Minus_triangle, s) 
+      \<Rightarrow>\<^bsup>mul_time (1 + s ''a'') + 6\<^esup> 
+      s(''a'' := 0,
+        ''b'' := 0,
+        ''c'' := 0,
+        ''d'' := 0,
+        ''triangle'' := triangle (s ''a''))"
+  unfolding IMP_Minus_triangle_def triangle_def 
+  by(force
+      intro: terminates_in_state_intro[OF Seq[OF Seq]]
+        IMP_minus_mul_correct)
+
+definition IMP_Minus_prod_encode where "IMP_Minus_prod_encode \<equiv>
+  ''prod_encode'' ::= (A (V ''a'')) ;;
+  ''a'' ::= ((V ''a'') \<oplus> (V ''b'')) ;;
+  IMP_Minus_triangle ;;
+  ''prod_encode'' ::= ((V ''triangle'') \<oplus> (V ''prod_encode'')) ;;
+  ''triangle'' ::= (A (N 0))"
+
+lemma IMP_Minus_prod_encode_correct: 
+  "(IMP_Minus_prod_encode, s) 
+      \<Rightarrow>\<^bsup>mul_time (1 + s ''a'' + s ''b'') + 14\<^esup> 
+      s(''a'' := 0,
+        ''b'' := 0,
+        ''c'' := 0,
+        ''d'' := 0,
+        ''triangle'' := 0,
+        ''prod_encode'' := prod_encode (s ''a'', s ''b''))"
+  unfolding IMP_Minus_prod_encode_def prod_encode_def
+  by(force
+      intro: terminates_in_state_intro[OF Seq[OF Seq]]
+        IMP_Minus_triangle_correct)
+
+fun prod_decode_aux_iterations :: "nat \<Rightarrow> nat \<Rightarrow> nat"
+  where "prod_decode_aux_iterations k m =
+    (if m \<le> k then 0 else Suc (prod_decode_aux_iterations (Suc k) (m - Suc k)))"
+
+declare prod_decode_aux_iterations.simps [simp del]
+
+definition prod_decode_aux_iteration where "prod_decode_aux_iteration \<equiv>
+  ''a'' ::= ((V ''a'') \<oplus> (N 1)) ;;
+  ''b'' ::= ((V ''b'') \<ominus> (V ''a'')) ;;
+  ''c'' ::= ((V ''b'') \<ominus> (V ''a''))"
+
+lemma prod_decode_aux_loop_correct: 
+  "s ''a'' = k \<Longrightarrow> s ''b'' = m \<Longrightarrow> s ''c'' = m - k 
+  \<Longrightarrow> (WHILE ''c'' \<noteq>0 DO prod_decode_aux_iteration, s) 
+      \<Rightarrow>\<^bsup>2 + 7 * prod_decode_aux_iterations (s ''a'') (s ''b'')\<^esup> 
+    s(''a'' := fst (prod_decode_aux (s ''a'') (s ''b''))
+         + snd (prod_decode_aux (s ''a'') (s ''b'')),
+      ''b'' := fst (prod_decode_aux (s ''a'') (s ''b'')),
+      ''c'' := 0)"
+proof(induction k m arbitrary: s rule: prod_decode_aux.induct)
+  case (1 k m)
+  then show ?case
+  proof(cases "m - k")
+    case 0
+    then show ?thesis
+      using 1 terminates_in_state_intro[OF Big_StepT.WhileFalse]
+      by(auto simp: fun_eq_iff prod_decode_aux.simps numeral_eq_Suc 
+          prod_decode_aux_iterations.simps)
+  next
+    case (Suc nat)
+
+    have first_iteration: "(prod_decode_aux_iteration, s) \<Rightarrow>\<^bsup> 6 \<^esup> 
+      s(''a'' := Suc k,
+        ''b'' := m - (Suc k),
+        ''c'' := (m - (Suc k)) - Suc k)"
+      unfolding prod_decode_aux_iteration_def
+      using \<open>s ''a'' = k\<close>  \<open>s ''b'' = m\<close>
+      by(auto 
+          simp: numeral_eq_Suc fun_eq_iff 
+          intro!: terminates_in_state_intro[OF Seq[OF Seq]])
+
+    show ?thesis
+      using terminates_in_state_intro[OF Big_StepT.WhileTrue[OF _ first_iteration "1.IH"]]
+        prod_decode_aux_iterations.simps[where ?k = "s ''a''"]
+        prod_decode_aux.simps[where ?k = "s ''a''"]
+        \<open>s ''a'' = k\<close>  \<open>s ''b'' = m\<close> \<open>s ''c'' = m - k\<close> \<open>m - k = Suc nat\<close>
+      by(auto simp: fun_eq_iff)
+  qed
+qed
+
+definition IMP_Minus_fst_nat where "IMP_Minus_fst_nat \<equiv>
+  ''b'' ::= (A (V ''a'')) ;; 
+  ''a'' ::= (A (N 0)) ;;
+  ''c'' ::= ((V ''b'') \<ominus> (V ''a'')) ;;
+  WHILE ''c'' \<noteq>0 DO prod_decode_aux_iteration ;;
+  ''fst_nat'' ::= (A (V ''b'')) ;;
+  ''a'' ::= (A (N 0)) ;;
+  ''b'' ::= (A (N 0))"
+
+lemma IMP_Minus_fst_nat_correct: 
+  "(IMP_Minus_fst_nat, s) 
+      \<Rightarrow>\<^bsup>14 + 7 * prod_decode_aux_iterations 0 (s ''a'')\<^esup> 
+    s(''a'' := 0,
+      ''b'' := 0,
+      ''c'' := 0,
+      ''fst_nat'' := fst_nat (s ''a''))"
+  unfolding IMP_Minus_fst_nat_def fst_nat_def prod_decode_def
+  by (force intro!: 
+      terminates_in_state_intro[OF Seq]
+      prod_decode_aux_loop_correct)
+
+definition IMP_Minus_snd_nat where "IMP_Minus_snd_nat \<equiv>
+  ''b'' ::= (A (V ''a'')) ;; 
+  ''a'' ::= (A (N 0)) ;;
+  ''c'' ::= ((V ''b'') \<ominus> (V ''a'')) ;;
+  WHILE ''c'' \<noteq>0 DO prod_decode_aux_iteration ;;
+  ''snd_nat'' ::= ((V ''a'') \<ominus> (V ''b'')) ;;
+  ''a'' ::= (A (N 0)) ;;
+  ''b'' ::= (A (N 0))"
+
+lemma IMP_Minus_snd_nat_correct: 
+  "(IMP_Minus_snd_nat, s) 
+      \<Rightarrow>\<^bsup>14 + 7 * prod_decode_aux_iterations 0 (s ''a'')\<^esup> 
+    s(''a'' := 0,
+      ''b'' := 0,
+      ''c'' := 0,
+      ''snd_nat'' := snd_nat (s ''a''))"
+  unfolding IMP_Minus_snd_nat_def snd_nat_def prod_decode_def
+  by (force intro!: 
+      terminates_in_state_intro[OF Seq]
+      prod_decode_aux_loop_correct)
+end
